update wip

core/ExtensionalUpdate.v
@@ -3,6 +3,7 @@ Require Import Net.
 Require Import Util.
 Require Import Omega.
 Require Import List.
+Require Import FunctionalExtensionality.
 Import ListNotations.
 
 Section SimpleUpdateFacts.
@@ -53,8 +54,8 @@ Section ExtensionalUpdate.
     forall i1 i2 update1 update2,
       Nth updates i1 update1 ->
       Nth updates i2 update2 ->
-      (forall h i d, huInput update1 h i d = huInput update2 h i d) ->
-      (forall h h' m d, huNet update1 h h' m d = huNet update2 h h' m d) ->
+      (forall h i d, huInput update1 h i d = huInput update2 h i d) /\
+      (forall h h' m d, huNet update1 h h' m d = huNet update2 h h' m d) /\
       (forall d, huReboot update1 d = huReboot update2 d).
   Variable updates_noop :
     forall i update,
@@ -63,6 +64,8 @@ Section ExtensionalUpdate.
   
   Variable first_update : handlerUpdate P.
   Variable first_update_first : Nth updates 0 first_update.
+
+  Definition multi_updates := updates.
 
   Instance one_update_params : SimpleUpdateParams P :=
     { updates := [first_update] }.
@@ -80,38 +83,152 @@ Section ExtensionalUpdate.
     snd (fst st) = snd (fst st') /\
     snd st = snd st'.
 
+  Lemma Nth_nth :
+    forall A (l : list A) n x y,
+      Nth l n x ->
+      nth n l y = x.
+  Proof.
+    induction 1; intuition.
+  Qed.
+
+  Lemma nth_Nth :
+    forall A n (l : list A) y,
+      n < length l ->
+      Nth l n (nth n l y).
+  Proof.
+    induction n; intros; destruct l; subst; simpl in *;
+    try omega; constructor; intuition.
+  Qed.
+
+  Lemma Nth_singleton :
+    forall A (x : A) y n,
+      Nth [x] n y ->
+      y = x.
+  Proof.
+    intros. inversion H; intuition. solve_by_inversion.
+  Qed.
+  
   Definition step_one_step_multi :
     forall sto sto' stm tr,
       reachable step_one step_u_init sto ->
+      reachable step_multi step_u_init stm ->
       step_one sto sto' tr ->
       equiv_except_handlers sto stm ->
       exists stm',
         equiv_except_handlers sto' stm' /\
         step_multi stm stm' tr.
   Proof.
-    intros. invcs H0.
+    intros. invcs H1.
     - destruct stm.
-      get_invariant updates_valid_inductive.
+      destruct p0.
+      copy_apply (inductive_invariant_true_in_reachable (@updates_valid_inductive _ _ _ params)) H0.
       unfold updates_valid in *. simpl in *.
       unfold equiv_except_handlers in *. simpl in *.
       intuition. subst.
       match goal with
         | |- context [(?x = _ /\ ?y = _)] =>
-          (exists (up, x, y))
+          (exists (n0, x, y))
       end.
       intuition.
-      destruct n.
-      simpl in *. subst. destruct p0. simpl in *. 
-      
-      exists (up, snd p0, snd ).
-      eexists; unfold equiv_except_handlers; simpl; intuition eauto.
-      pose proof .
-      copy_apply H0 H.
+      assert (Nth multi_updates (n0 (pDst p))
+                  (nth (n0 (pDst p)) multi_updates first_update))
+      by
+        (match goal with
+           | H : forall _, _ \/ _ |- _ =>
+             specialize (H (pDst p))
+         end; intuition; eauto using nth_Nth;
+         repeat find_rewrite;
+         erewrite Nth_nth; eauto).
+      eapply SU_deliver with (handlers0 := nth (n0 (pDst p)) multi_updates first_update);
+        simpl in *; eauto; unfold multi_updates in *.
+      find_apply_lem_hyp Nth_singleton. subst.
+      find_reverse_rewrite.
+      eapply all_handlers_ext_equal; eauto.
+    - destruct stm. destruct p.
+      copy_apply (inductive_invariant_true_in_reachable (@updates_valid_inductive _ _ _ params)) H0.
+      unfold updates_valid in *. simpl in *.
+      unfold equiv_except_handlers in *. simpl in *.
+      intuition. subst.
+      match goal with
+        | |- context [(?x = _ /\ ?y = _)] =>
+          (exists (n0, x, y))
+      end.
+      intuition.
+      assert (Nth multi_updates (n0 h)
+                  (nth (n0 h) multi_updates first_update))
+      by
+        (match goal with
+           | H : forall _, _ \/ _ |- _ =>
+             specialize (H h)
+         end; intuition; eauto using nth_Nth;
+         repeat find_rewrite;
+         erewrite Nth_nth; eauto).
+      eapply SU_input with (handlers0 := nth (n0 h) multi_updates first_update);
+        simpl in *; eauto; unfold multi_updates in *.
+      find_apply_lem_hyp Nth_singleton. subst.
+      find_reverse_rewrite.
+      eapply all_handlers_ext_equal; eauto.
+    - destruct stm. destruct p0.
+      unfold equiv_except_handlers in *. simpl in *.
+      intuition. subst.
+      match goal with
+        | |- context [(?x = _ /\ ?y = _)] =>
+          (exists (n0, x, y))
+      end.
+      intuition.
+      solve [econstructor; eauto].
+    - destruct stm. destruct p0.
+      unfold equiv_except_handlers in *. simpl in *.
+      intuition. subst.
+      match goal with
+        | |- context [(?x = _ /\ ?y = _)] =>
+          (exists (n0, x, y))
+      end.
+      intuition.
+      solve [econstructor; eauto].
+    - destruct stm. destruct p.
+      unfold equiv_except_handlers in *. simpl in *.
+      intuition. subst.
+      match goal with
+        | |- context [(?x = _ /\ ?y = _)] =>
+          (exists (n0, x, y))
+      end.
+      intuition.
+      solve [econstructor; eauto].
+    - destruct stm. destruct p.
+      copy_apply (inductive_invariant_true_in_reachable (@updates_valid_inductive _ _ _ params)) H0.
+      unfold updates_valid in *. simpl in *.
+      unfold equiv_except_handlers in *. simpl in *.
+      intuition. subst.
+      match goal with
+        | |- context [(?x = _ /\ ?y = _)] =>
+          (exists (n0, x, y))
+      end.
+      intuition.
+      assert (Nth multi_updates (n0 h)
+                  (nth (n0 h) multi_updates first_update))
+      by
+        (match goal with
+           | H : forall _, _ \/ _ |- _ =>
+             specialize (H h)
+         end; intuition; eauto using nth_Nth;
+         repeat find_rewrite;
+         erewrite Nth_nth; eauto).
+      eapply SU_reboot with (handlers0 := nth (n0 h) multi_updates first_update);
+        simpl in *; eauto; unfold multi_updates in *.
+      find_apply_lem_hyp Nth_singleton. subst.
+      copy_eapply_prop_hyp huReboot @Nth; [|apply first_update_first].
+      intuition.
+      f_equal. apply functional_extensionality.
+      intros.
+      find_higher_order_rewrite. auto.
+    - match goal with
+        | H : Nth _ _ _ |- _ =>
+          inversion H
+      end. solve_by_inversion.
+  Qed.
 
-      assert (exists handlers, Nth updates (up (pDst p)) handlers).
-      + 
-    
-  
+      
   Definition inv_holds_one :=
     forall st' tr,
       @step_u_star _ _ _ one_update_params step_u_init st' tr ->
